11 12

assignments/12/P03.v
@@ -13,30 +13,51 @@ Require Export P02.
 *)
 
 Definition halve : tm :=
-  FILL_IN_HERE.
+  tfix (tabs Halve (TArrow TNat TNat) (tabs X TNat 
+    (tif0 (tvar X)
+      (tnat 0)
+      (tif0 (tpred (tvar X))
+        (tnat 0)
+        (tsucc (tapp (tvar Halve) (tpred (tpred (tvar X)))))
+      )
+    )
+  )).
 
 Example halve_type: empty |- halve \in TArrow TNat TNat.
 Proof.
-  (* unfold halve; eauto 10. *)
-  exact FILL_IN_HERE.
+  unfold halve; eauto 10.
 Qed.
 
 Example halve_10: tapp halve (tnat 10) ==>* tnat 5.
 Proof.
-  (* unfold halve; normalize. *)
-  exact FILL_IN_HERE.
+  unfold halve; normalize.
 Qed.
 
 Example halve_11: tapp halve (tnat 11) ==>* tnat 5.
 Proof.
-  (* unfold halve; normalize. *)
-  exact FILL_IN_HERE.
+  unfold halve; normalize.
 Qed.
 
 
 Theorem halve_correct: forall n,
    tapp halve (tnat (n+n)) ==>* tnat n.
 Proof.
-  exact FILL_IN_HERE.
+  intros n. induction n.
+  - simpl. unfold halve. normalize.
+  - eapply multi_step. eapply ST_AppFix; eauto.
+    eapply multi_step. eapply ST_App1; eauto.
+    eapply multi_step. simpl. eapply ST_AppAbs; eauto.
+    eapply multi_step. simpl. eapply ST_If0Nonzero.
+    eapply multi_step. eapply ST_If01; eauto. simpl. rewrite <- plus_n_Sm.
+    eapply multi_step. eapply ST_If0Nonzero.
+    eapply multi_step. eapply ST_Succ1. eapply ST_App2; eauto.
+    eapply multi_step. eapply ST_Succ1. eapply ST_App2; eauto.
+    simpl.
+    assert (forall t1 t2, t1 ==>* t2 -> tsucc t1 ==>* tsucc t2).
+    { intros t1 t2 H. induction H; eauto. }
+    apply H in IHn. eapply multi_trans. unfold halve in IHn. apply IHn.
+    eapply multi_step. eauto. apply multi_refl.
+    
+  
 Qed.
 
