assignments/10/P06.v
@@ -12,11 +12,19 @@ Require Export P05.
    You can use the following intro pattern:
      destruct ... as [ | [? [? ?]]].
 *)
-
+Hint Constructors cstep.
 Theorem cimp_strong_progress : forall c st,
   c = SKIP \/ 
   exists c' st', c / st ==> c' / st'.
 Proof.
-  exact FILL_IN_HERE.
+  remember (aexp_strong_progress) as HA.
+  remember (bexp_strong_progress) as HB.
+  intros c st. induction c; try eauto; right.
+  try destruct (HA st a) as [HA'|HA']; try inversion HA'; subst; eauto.
+  try destruct IHc1 as [Hc1|Hc1]; try destruct IHc2 as [Hc2|Hc2]; try inversion Hc1; try inversion Hc2; try inversion H;
+  subst; eauto.
+  try destruct (HB st b) as [[HB'|HB']|HB']; try inversion HB'; subst; try eauto.
+  try destruct IHc1 as [Hc1|Hc1]; try destruct IHc2 as [Hc2|Hc2]; try inversion Hc1; try inversion Hc2; try inversion H;
+  subst; try inversion H0; eauto.
 Qed.
 
